Bytestring/ByteArray.lean
@@ -10,7 +10,7 @@ theorem ByteArray.size_data {a : ByteArray} :
 @[simp]
 theorem ByteArray.data_append {l l' : ByteArray} :
     (l ++ l').data = l.data ++ l'.data := by
-  simp [append_eq_copySlice, copySlice, ← ByteArray.size_data, ← Array.append_assoc]
+  simp [append_eq_copySlice, copySlice, ← ByteArray.size_data, - Array.append_assoc]
 
 @[simp]
 theorem ByteArray.data_push {a : ByteArray} {b : UInt8} :
@@ -44,7 +44,7 @@ theorem List.toByteArray_append {l l' : List UInt8} :
   simp
 
 @[simp]
-theorem List.toByteArray_empty : List.toByteArray [] = ByteArray.empty := rfl
+theorem List.toByteArray_nil : List.toByteArray [] = ByteArray.empty := rfl
 
 @[simp]
 theorem ByteArray.empty_append {b : ByteArray} : ByteArray.empty ++ b = b := by
@@ -56,7 +56,7 @@ theorem ByteArray.append_empty {b : ByteArray} : b ++ ByteArray.empty = b := by
   ext1
   simp
 
-@[simp]
+@[simp, grind]
 theorem ByteArray.size_append {a b : ByteArray} : (a ++ b).size = a.size + b.size := by
   simp [← size_data]
 
@@ -69,6 +69,7 @@ theorem ByteArray.size_eq_zero_iff {a : ByteArray} : a.size = 0 ↔ a = ByteArra
 theorem ByteArray.getElem_eq_getElem_data {a : ByteArray} {i : Nat} {h : i < a.size} :
     a[i] = a.data[i]'(by simpa [← size_data]) := rfl
 
+@[simp]
 theorem ByteArray.getElem_append_left {i : Nat} {a b : ByteArray} {h : i < (a ++ b).size}
     (hlt : i < a.size) : (a ++ b)[i] = a[i] := by
   simp only [getElem_eq_getElem_data, data_append]
@@ -84,3 +85,73 @@ theorem ByteArray.getElem_append_right {i : Nat} {a b : ByteArray} {h : i < (a +
 theorem List.getElem_toByteArray {l : List UInt8} {i : Nat} {h : i < l.toByteArray.size} :
     l.toByteArray[i] = l[i]'(by simp_all) := by
   simp [ByteArray.getElem_eq_getElem_data]
+
+def ByteArray.drop (b : ByteArray) (i : Nat) : ByteArray :=
+  b.extract i b.size
+
+@[simp]
+theorem ByteArray.drop_eq_extract {b : ByteArray} {i : Nat} :
+  b.drop i = b.extract i b.size := rfl
+
+@[simp]
+theorem ByteArray.data_extract {a : ByteArray} {b e : Nat} :
+    (a.extract b e).data = a.data.extract b e := by
+  simp [extract, copySlice]
+  grind
+
+@[simp]
+theorem ByteArray.size_extract {a : ByteArray} {b e : Nat} :
+    (a.extract b e).size = min e a.size - b := by
+  simp [← size_data]
+
+@[simp]
+theorem ByteArray.extract_size_size {b : ByteArray} : b.extract b.size b.size = ByteArray.empty := by
+  ext1
+  simp
+
+@[simp]
+theorem ByteArray.extract_eq_empty_iff {b : ByteArray} {i j : Nat} : b.extract i j = ByteArray.empty ↔ min j b.size ≤ i := by
+  rw [← size_eq_zero_iff, size_extract]
+  omega
+
+@[simp]
+theorem ByteArray.extract_zero_size {b : ByteArray} : b.extract 0 b.size = b := by
+  ext1
+  simp
+
+@[simp]
+theorem ByteArray.append_eq_empty_iff {a b : ByteArray} :
+    a ++ b = ByteArray.empty ↔ a = ByteArray.empty ∧ b = ByteArray.empty := by
+  simp [← size_eq_zero_iff, size_append]
+
+@[simp]
+theorem List.toByteArray_eq_empty {l : List UInt8} :
+    l.toByteArray = ByteArray.empty ↔ l = [] := by
+  simp [← ByteArray.size_eq_zero_iff]
+
+theorem ByteArray.append_right_inj {ys₁ ys₂ : ByteArray} (xs : ByteArray) :
+    xs ++ ys₁ = xs ++ ys₂ ↔ ys₁ = ys₂ := by
+  simp [ByteArray.ext_iff, Array.append_right_inj]
+
+@[simp]
+theorem ByteArray.extract_append_extract {a : ByteArray} {i j k : Nat} :
+    a.extract i j ++ a.extract j k = a.extract (min i j) (max j k) := by
+  ext1
+  simp
+
+theorem ByteArray.extract_eq_extract_append_extract {a : ByteArray} {i k : Nat} (j : Nat)
+    (hi : i ≤ j) (hk : j ≤ k) :
+    a.extract i k = a.extract i j ++ a.extract j k := by
+  simp; grind
+
+--  {α : Type u_1} {xs₁ xs₂ ys₁ ys₂ : Array α} (h : xs₁ ++ ys₁ = xs₂ ++ ys₂) (hl : xs₁.size = xs₂.size) : xs₁ = xs₂
+
+theorem ByteArray.append_inj_left {xs₁ xs₂ ys₁ ys₂ : ByteArray} (h : xs₁ ++ ys₁ = xs₂ ++ ys₂) (hl : xs₁.size = xs₂.size) : xs₁ = xs₂ := by
+  simp only [ByteArray.ext_iff, ← ByteArray.size_data, ByteArray.data_append] at *
+  exact Array.append_inj_left h hl
+
+theorem ByteArray.extract_append_eq_right {a b : ByteArray} {i : Nat} (hi : i = a.size) :
+    (a ++ b).extract i (a ++ b).size = b := by
+  subst hi
+  ext1
+  simp [← size_data]
